---
title: "eecenter"
format: pdf
---

$$
T_{ij}=(e_ie_j'+e_je_i')-\frac{1}{n}(e_i+e_j)e'-\frac{1}{n}e(e_i+e_j)'+\frac{2}{n^2}ee'
$$
$$
T_{kl}=(e_ke_l'+e_le_k')-\frac{1}{n}(e_k+e_l)e'-\frac{1}{n}e(e_k+e_l)'+\frac{2}{n^2}ee'
$$
Start over
$$
\text{tr}\ JE_{ij}JJE_{kl}J=\text{tr}\ E_{ij}JE_{kl}J
$$
$$
E_{ij}J=(e_ie_j'+e_je_i')(I-\frac{1}{n}ee')=(e_ie_j'+e_je_i')-\frac{1}{n}(e_i+e_j)e'
$$
\begin{align}
\text{tr}\ E_{ij}JE_{kl}J=
&\text{tr}\ (e_ie_j'+e_je_i')(e_ke_l'+e_le_k')-\\
&\frac{1}{n}\text{tr}\ (e_ie_j'+e_je_i')(e_k+e_l)e'-\\
&\frac{1}{n}\text{tr}\ (e_i+e_j)e'(e_ke_l'+e_le_k')+\\
&\frac{1}{n^2}\text{tr}\ (e_i+e_j)e'(e_k+e_l)e'
\end{align}

\begin{equation}
\text{tr}\ E_{ij}JE_{kl}J=
2(\delta^{ik}\delta^{jl}+\delta^{il}\delta^{jk})-
\frac{2}{n}(\delta^{ik}+\delta^{il}+\delta^{jk}+\delta^{jl})+
\frac{4}{n^2}
\end{equation}

$$
\frac14\text{tr}\ T_{ij}T_{kl}=
\begin{cases}
\frac12-\frac{1}{n}+\frac{1}{n^2}&\text{two indices in common},\\
-\frac{1}{2n}+\frac{1}{n^2}&\text{one index in common},\\
\frac{1}{n^2}&\text{no indices in common}
\end{cases}
$$

